Add files via upload
We have finished the definition of the syntactic derivative for the "computable polynomials". Our next step is to prove some properties of well-behavior of our definition.

FirstAttempt.thy
@@ -2,27 +2,27 @@ theory FirstAttempt
   imports 
 Main
 "../afp-2017-10-18/thys/Polynomials/Polynomials"
+"HOL.Real"
 
 begin
 
 context linorder
 begin
-
 text{* Useful definitions from the AFP entry on Polynomials. For specific examples see the 
 document "ExplorePolinoms.thy" and the end of this file:
-  · 'v monom_list = "('v \<times> nat)list" 
-  · ('v,'a)poly = "('v monom \<times> 'a)list" 
+  · 'v monom_list = "('v \<times> nat)list"  
   · 'v monom = Collect monom_inv
   · The function monom_inv, referred above tests three things:
       - That all the powers are greater than or equal to 1.
       - That all the variables are different.
       - That all variables appear ordered.
 OBSERVATION: Because of the way monomials are built, we need to ensure that our derivatives
-respect the function "monom_inv".
+respect the function "monom_inv". This is what we do in this context.
 *}
 
 (* This abbreviation tests if the first argument is a variable appearing in the monomial. *)
-abbreviation IsNotVar :: "'v \<Rightarrow> 'v monom_list \<Rightarrow> bool"   where "IsNotVar x ml \<equiv> (x \<notin> fst ` set ml)"
+abbreviation IsNotVar :: "'a \<Rightarrow> 'a monom_list \<Rightarrow> bool" 
+  where "IsNotVar x ml \<equiv> (x \<notin> fst ` set ml)"
 
 (* This terms are here so I can explicitly see how some operations in the abbreviation above work.*)
 value "snd ` set [(0::int,1::int),(2,3)] "
@@ -32,18 +32,30 @@ term "op `"
 with exponent 1, otherwise we substract one from the exponent i.e. 
   - downExp x xy\<^sup>2z = y\<^sup>2z 
   - downExp x x\<^sup>4y\<^sup>2z = x\<^sup>3y\<^sup>2z *)
-fun downExp :: "'v \<Rightarrow> 'v monom_list \<Rightarrow> 'v monom_list" where
+fun downExp :: "'a \<Rightarrow> 'a monom_list \<Rightarrow> 'a monom_list" where
 "downExp x [] = []"|
-"downExp x ((z,n) # tail) = (if x = z then (if n=1 then tail else (z,n-1) # tail) else (z,n) # downExp x tail)"
+"downExp x ((z,n) # tail) = 
+          (if x = z then (if n=1 then tail else (z,n-1) # tail) else (z,n) # downExp x tail)"
 
 (* Operation in the coefficients. Separately, we return the coefficient. *)
-fun derivCoeffMonomList :: "'v \<Rightarrow> 'v monom_list \<Rightarrow> nat" where
+fun derivCoeffMonomList :: "'a \<Rightarrow> 'a monom_list \<Rightarrow> nat" where
 "derivCoeffMonomList x [] = 0"|
 "derivCoeffMonomList x ((z,n) # tail) = (if x = z then n else derivCoeffMonomList x tail)"
 
 (* The derivative on a monomList returns a pair of a coefficient and a monomList. *)
-definition derivMonomList :: "'v \<Rightarrow> 'v monom_list \<Rightarrow> (nat \<times> 'v monom_list)" where
-  "derivMonomList x ml = (if IsNotVar x ml then (0,[]) else (derivCoeffMonomList x ml,downExp x ml))"
+definition derivMonomList :: "'a \<Rightarrow> 'a monom_list \<Rightarrow> (nat \<times> 'a monom_list)" where
+  "derivMonomList x ml = 
+          (if IsNotVar x ml then (0,[]) else (derivCoeffMonomList x ml,downExp x ml))"
+
+(* Some values to quickly check that our derivatives for monomials work as expected. *)
+value "derivMonomList 1 ([]::(int \<times> nat)list)"
+value "derivMonomList 1 [(1::int,1::nat)]"
+value "derivMonomList 0 [(0::int,1::nat),(2,3)]"
+value "derivMonomList 4 [(0::int,1::nat),(2,3)]"
+value "derivMonomList 4 [(0::int,1::nat),(2,3),(4,2)]"
+value "derivMonomList 4 [(0::int,1::nat),(2,3),(4,1)]"
+value "derivMonomList 4 [(0::int,1::nat),(2,3),(4,0)]"
+(* Notice this last input does not satisfy "monom_inv". *)
 
 (* \<partial> x 0 = 0 *)
 lemma derivZeroMonomList [simp]: "derivMonomList x [] = (0,[])"
@@ -67,36 +79,167 @@ lemma derivOfConst [simp]: "IsNotVar x ml \<Longrightarrow> derivMonomList x ml 
 lemma [simp]: "monom_inv [] = True"
   by (simp add: monom_inv_def)
 
-(* Stucked with this proof. For now... Not sure if necessary. *)
-lemma derivReturnsMonoms : "monom_inv list \<Longrightarrow> monom_inv (snd (derivMonomList x list))"
-  oops
+(* Monomials do not have variables to the zeroth power. *)
+lemma noZeroExpInMonoms: "monom_inv (monlist) \<Longrightarrow> (x, 0) \<notin> set (monlist)"
+proof
+  assume a:"monom_inv (monlist)"
+  from a have b:"\<forall>(x, n) \<in> set (monlist). 1 \<le> n" by(simp add: monom_inv_def)
+  assume c: "(x, 0) \<in> set (monlist)" --"to get a contradiction"
+  from c and b have d: "1 \<le> (0::nat)" by (force)
+  thus False by linarith 
+qed
 
+text{* We begin a proof to see that the derivative operator on monomials respects the 
+predicate "monom_inv". For this we show three things: 
+  - That all variables appear ordered.
+  - That all the variables are different.
+  - That all the powers are greater than or equal to 1.
+*}
+
+(* Lemmas for the first condition. *)
+lemma downExpRespectsSortedness: "sorted (map fst list) \<Longrightarrow> sorted (map fst (downExp x list))"
+  apply(induction list, auto)
+    apply (simp add: local.sorted_Cons)
+    apply (smt downExp.elims fst_conv insert_iff list.simps(15) list.simps(9) 
+local.sorted_Cons local.sorted_many_eq)
+    apply (smt downExp.elims fst_conv insert_iff list.simps(15) list.simps(9) 
+local.sorted_Cons local.sorted_many)
+  done
+
+lemma fstCondMonomInv: "\<forall> list. monom_inv (list) \<longrightarrow> sorted (map fst (downExp x list))"
+  apply(auto simp: monom_inv_def)
+  using downExpRespectsSortedness by blast
+
+(* Lemmas for the second condition. *)
+lemma[simp]: "IsNotVar x list \<Longrightarrow> downExp x list = list"
+  apply(induction list rule: downExp.induct, auto)
+  done
+  
+lemma downExpPreservesVars: "set (map fst (downExp x list)) \<subseteq> set (map fst list)"
+  apply(induction list rule: downExp.induct, auto)
+  done
+  
+lemma downExpRespectsDistinct: "distinct (map fst list) \<Longrightarrow> distinct (map fst (downExp x list))"
+  apply(induction list rule: downExp.induct, simp)
+  apply(simp)
+  apply(rule impI)
+  by (metis downExpPreservesVars list.set_map subsetCE)
+
+lemma sndCondMonomInv: "\<forall> list. monom_inv (list) \<longrightarrow> distinct (map fst (downExp x list))"
+  by (simp add: downExpRespectsDistinct local.monom_inv_def)
+  
+(* Lemmas for the third condition. *)
+lemma downExpRespectsPows: "(\<forall> (var,num) \<in> set list. 1 \<le> num) \<Longrightarrow> (x,n) \<in> set list \<Longrightarrow>
+ \<forall> (var,num) \<in> set (downExp x list). 1 \<le> num"
+ apply(induction list rule: downExp.induct, simp)
+ by (smt case_prod_conv diff_is_0_eq' downExp.simps(2) less_one 
+     linorder_class.not_le list.set_intros(1) list.set_intros(2) 
+     order_class.order.not_eq_order_implies_strict set_ConsD zero_less_diff)
+
+lemma thrdCondMonomInv: "monom_inv (list) \<Longrightarrow> (x,n) \<in> set list \<Longrightarrow>
+ (\<forall> (var,num) \<in> set (downExp x list). 1 \<le> num)"
+ apply(simp add: monom_inv_def)
+ by (metis (no_types, lifting) One_nat_def case_prodI2 downExpRespectsPows old.prod.case)
+ 
+ 
 (* According to Isabelle, she needs this as a theorem to do the lifting to monomials. *)
-lemma derivReturnsMonoms : "monom_inv list \<Longrightarrow> (x,n) \<in> set list \<Longrightarrow> monom_inv (downExp x list)"
-  apply (induction list rule: downExp.induct)
-   apply(simp)
-  oops
-
-(* Previous lemma necessary to do the lifting, and be able to define derivatives for polynomials. *)
-lift_definition derivMonom :: "'v \<Rightarrow> 'v::linorder monom \<Rightarrow> (nat \<times>'v monom)" is derivMonomList
-  apply(auto simp: derivMonomList_def)
-  using linorder_class.monom_inv_def apply fastforce
-
-(* Derivative on polynomials with respect to a variable, it still working it out... *)
-fun deriv :: "'a \<Rightarrow> ('v,'a)poly \<Rightarrow> ('v,'a)poly" where
-"deriv x [] = zero_poly"|
-"deriv x [(m, coef)] = (if x \<notin> set (map fst ` m) then zero_poly else zero_poly)"
-
+theorem derivReturnsMonoms :
+"\<forall> list. monom_inv list \<longrightarrow> (x,n) \<in> set list \<longrightarrow> monom_inv (downExp x list)"
+proof
+  fix list
+  show "monom_inv list \<longrightarrow> (x,n) \<in> set list \<longrightarrow> monom_inv (downExp x list)"
+    proof
+    assume hip1:"monom_inv list"
+    from this have sorted:"sorted (map fst (downExp x list))" by (auto simp: fstCondMonomInv)
+    from hip1 have distinct:"distinct (map fst (downExp x list))" by (auto simp: sndCondMonomInv)
+    show "(x, n) \<in> set list \<longrightarrow> monom_inv (downExp x list)"
+      proof
+      assume hip2:"(x,n) \<in> set list"
+      from hip1 and hip2 have powers: "(\<forall> (var,num) \<in> set (downExp x list). 1 \<le> num)"
+      using thrdCondMonomInv by blast
+      from sorted distinct and powers show "monom_inv (downExp x list)" 
+      by (auto simp: monom_inv_def)
+      qed
+    qed
+qed
+    
 end
 
-(* Some values to quickly check that our derivatives for monomials work as expected. *)
-value "derivMonomList 1 ([]::(int \<times> nat)list)"
-value "derivMonomList 1 [(1::int,1::nat)]"
-value "derivMonomList 0 [(0::int,1::nat),(2,3)]"
-value "derivMonomList 4 [(0::int,1::nat),(2,3)]"
-value "derivMonomList 4 [(0::int,1::nat),(2,3),(4,2)]"
-value "derivMonomList 4 [(0::int,1::nat),(2,3),(4,1)]"
-value "derivMonomList 4 [(0::int,1::nat),(2,3),(4,0)]"
-(* Notice this last input does not satisfy "monom_inv". *)
+(* Previous lemma necessary to do the lifting. In turn, the lifting is necessary to define 
+derivatives for polynomials. *)
+lift_definition derivMonom :: "'a \<Rightarrow> 'a::linorder monom \<Rightarrow> (nat \<times>'a monom)" is derivMonomList
+  apply(transfer, auto simp: derivMonomList_def)
+  apply(simp add: derivReturnsMonoms)
+  done
+
+text{* Reminders for what comes next: 
+  · ('v,'a)poly = "('v monom \<times> 'a)list"
+  · derivMonom :: "'a \<Rightarrow> 'a monom \<Rightarrow> (nat \<times> 'a monom)" 
+  · poly_inv p \<equiv> (\<forall> c \<in> snd ` set p. c \<noteq> 0) \<and> distinct (map fst p)" *}
+  
+(* Exploring the locales to find a function "\<cdot>: nat \<Rightarrow> ('a::monoid_add) \<Rightarrow> 'a" that returns an
+element "x:'a" scaled as many times as "n:nat", i.e. it returns "n\<cdot>x=x+x+x+\<dots>+x".  *)
+  print_locales
+  thm ab_semigroup_add_class_def
+  thm ab_semigroup_add_axioms
+  thm plus_class_def
+
+(* As suggested by Andreas Lochbihler, we use the compow function in Nat.thy to define our
+scaling function. *)
+  term "op ^^"
+  term "compow 2 (2::int)"
+  term "(2::int)^^2 "
+
+  definition natScale :: "nat \<Rightarrow> ('a::semiring_0) \<Rightarrow> 'a" where
+  "natScale n x = ((plus x) ^^ n) 0"
+  
+  value "natScale 6 (-3::real)" 
+
+(* Derivative on polynomials with respect to a variable. *)
+fun deriv :: "('v::linorder) \<Rightarrow> ('v,'a:: semiring_0)poly \<Rightarrow> ('v,'a)poly" where
+"deriv x [] = zero_poly"|
+"deriv x [(mon, coef)] = (if (fst (derivMonom x mon)) = 0 then zero_poly else [(snd (derivMonom x mon),natScale (fst (derivMonom x mon)) coef)])"|
+"deriv x (headMonom # tailMonom) = (deriv x [headMonom]) @ (deriv x tailMonom)"
+
+(* Derivative on polynomials: syntactic version. *)
+fun derivList :: "('v::linorder) \<Rightarrow> ('v monom_list \<times> 'a:: semiring_0)list \<Rightarrow> ('v monom_list \<times> 'a)list" where
+"derivList x [] = []"|
+"derivList x [(mon, coef)] = (if (derivCoeffMonomList x mon) = 0 then [] else 
+[((if (IsNotVar x mon) then [] else downExp x mon),natScale (derivCoeffMonomList x mon) coef)])"|
+"derivList x (headMonom # tailMonom) = (derivList x [headMonom]) @ (derivList x tailMonom)"
+
+(* \<real>[x,y,z,w] \<ni> P(x,y,z,w) = 2 + w + 3xyz + 3x\<^sup>2 + y\<^sup>2z + 5z\<^sup>3. *)
+term "[([],2),([((1::int),1),(2,1),(3,1)],3::real),([(1,2::nat)],3),([(2,2),(3,1)],1),([(3,3)],5),([(4,1)],1)]"
+term "(deriv 1 [(Abs_monom [((1::int),1),(2,1),(3,1)],3::real)])::(int,real)poly"
+(* \<partial> x P(x,y,z,w) = 3yz + 6x. *)
+value "(derivList 1 [([],2),([((1::int),1),(2,1),(3,1)],3::real),([(1,2)],3),([(2,2),(3,1)],1),([(3,3)],5),([(4,1)],1)])"
+(* \<partial> y P(x,y,z,w) = 3xz + 2yz. *)
+value "(derivList 2 [([],2),([((1::int),1),(2,1),(3,1)],3::real),([(1,2)],3),([(2,2),(3,1)],1),([(3,3)],5),([(4,1)],1)])"
+(* \<partial> z P(x,y,z,w) = 3xy + y\<^sup>2 + 15z\<^sup>2. *)
+value "(derivList 3 [([],2),([((1::int),1),(2,1),(3,1)],3::real),([(1,2)],3),([(2,2),(3,1)],1),([(3,3)],5),([(4,1)],1)])"
+(* \<partial> w P(x,y,z,w) = 1. *)
+value "(derivList 4 [([],2),([((1::int),1),(2,1),(3,1)],3::real),([(1,2)],3),([(2,2),(3,1)],1),([(3,3)],5),([(4,1)],1)])"
+(* \<partial> v P(x,y,z,w) = 0. *)
+value "(derivList 5 [([],2),([((1::int),1),(2,1),(3,1)],3::real),([(1,2)],3),([(2,2),(3,1)],1),([(3,3)],5),([(4,1)],1)])"
+
+lemma "deriv x (poly_add p q) = poly_add (deriv x p) (deriv x q)"
+apply(induction p rule: deriv.induct)
+apply(simp add: poly_zero_add poly_add.simps(1))
+apply(simp)
+oops
+
+
+lemma "set (deriv x (poly_add p q)) = set ((deriv x p) @ (deriv x q))"
+apply(simp)
+oops
+
+
+
+
+
+
+declare [[show_types]]
+declare [[show_sorts]]
+
 
 end
